[michocoq] Fix a bug in the typer
Type-checking a mutez literal now fails in case of overflow.

src/michocoq/int64bv.v
@@ -25,6 +25,8 @@
 Require Import Bvector.
 Require Import ZArith.
 Require Import Zdigits.
+Require Import Lia.
+Require error.
 
 Definition int64 := Bvector 64.
 
@@ -32,18 +34,142 @@ Definition sign : int64 -> bool := Bsign 63.
 
 Definition to_Z : int64 -> Z := two_compl_value 63.
 
-Definition of_Z : Z -> int64 := Z_to_two_compl 63.
+Lemma to_Z_lower_bound : forall b : int64, (- two_power_nat 63 <= to_Z b)%Z.
+Proof.
+  unfold int64, to_Z.
+  generalize 63.
+  intros n b.
+  refine (@VectorDef.caseS
+            _
+            (fun n b => - two_power_nat n <= two_compl_value n b)%Z
+            _ n b).
+  clear n b.
+  intros b n t.
+  simpl.
+  generalize b; clear b.
+  induction t.
+  + simpl.
+    unfold eq_rec_r.
+    simpl.
+    intro b; destruct b; simpl; omega.
+  + simpl two_compl_value.
+    unfold eq_rec_r.
+    simpl.
+    specialize (IHt h).
+    generalize IHt; clear IHt.
+    destruct (two_compl_value n (h :: t)).
+    * destruct b; simpl; nia.
+    * destruct b; simpl; nia.
+    * generalize (shift_nat n 1); intro p0; simpl.
+      destruct b; simpl; try nia.
+      apply Pos2Z.neg_le_neg.
+      unfold "<="%Z in IHt.
+      unfold "?="%Z in IHt.
+      rewrite <- Pos.compare_antisym in IHt.
+      change (p <= p0)%positive in IHt.
+      transitivity (p~0)%positive.
+      -- rewrite <- Pos.succ_pred_double.
+         lia.
+      -- nia.
+Qed.
+
+Lemma to_Z_upper_bound : forall b : int64, (to_Z b < two_power_nat 63)%Z.
+  unfold int64, to_Z.
+  generalize 63.
+  intros n b.
+  refine (@VectorDef.caseS
+            _
+            (fun n b => two_compl_value n b < two_power_nat n)%Z
+            _ n b).
+  clear n b.
+  intros b n t.
+  generalize b; clear b.
+  induction t.
+  + unfold two_power_nat.
+    simpl.
+    unfold eq_rec_r.
+    simpl.
+    intro b; destruct b; simpl; omega.
+  + simpl two_compl_value.
+    unfold eq_rec_r.
+    simpl.
+    specialize (IHt h).
+    generalize IHt; clear IHt.
+    unfold two_power_nat.
+    destruct (two_compl_value n (h :: t)).
+    * destruct b; simpl; nia.
+    * destruct b; simpl; nia.
+    * generalize (shift_nat n 1); intro p0; simpl.
+      destruct b; simpl; nia.
+Qed.
+
+Definition of_Z_unsafe : Z -> int64 := Z_to_two_compl 63.
+
+Definition of_Z_safe (z : Z) :
+  ((z >=? - two_power_nat 63) && (z <? two_power_nat 63))%Z = true -> int64 :=
+  fun _ => of_Z_unsafe z.
+
+Definition of_Z (z : Z) : error.M int64 :=
+  if ((z >=? - two_power_nat 63) && (z <? two_power_nat 63))%bool%Z
+  then
+    error.Return (of_Z_unsafe z)
+  else
+    error.Failed _ error.Overflow.
+
+Lemma of_Z_safe_is_of_Z z H : of_Z z = error.Return (of_Z_safe z H).
+Proof.
+  unfold of_Z, of_Z_safe.
+  rewrite H.
+  reflexivity.
+Qed.
 
 Definition int64_inversion (b : int64) : exists a v, b = Bcons a 63 v :=
   match b in Vector.t _ (S _) return exists a v, b = Bcons a _ v with
   | Vector.cons _ a _ v => ex_intro _ a (ex_intro _ v eq_refl)
   end.
 
-Lemma of_Z_to_Z b : of_Z (to_Z b) = b.
+Lemma of_Z_to_Z_eqv z b : to_Z b = z <-> of_Z z = error.Return b.
 Proof.
-  destruct (int64_inversion b) as (a, (v, H)).
-  rewrite H.
-  apply two_compl_to_Z_to_two_compl.
+  unfold of_Z, to_Z.
+  split.
+  - intro; subst z.
+    destruct (int64_inversion b) as (a, (v, H)).
+    rewrite H.
+    unfold of_Z_unsafe.
+    rewrite two_compl_to_Z_to_two_compl.
+    rewrite <- H; clear H.
+    assert ((two_compl_value 63 b >=? - two_power_nat 63)%Z = true) as Hlow.
+    + rewrite Z.geb_le.
+      apply to_Z_lower_bound.
+    + rewrite Hlow; clear Hlow.
+      assert ((two_compl_value 63 b <? two_power_nat 63)%Z = true) as Hhigh.
+      * rewrite Z.ltb_lt.
+        apply to_Z_upper_bound.
+      * rewrite Hhigh; clear Hhigh.
+        reflexivity.
+  - intro H.
+    case_eq ((z >=? - two_power_nat 63) && (z <? two_power_nat 63))%Z.
+    + intro Hcond.
+      rewrite Hcond in H.
+      apply (f_equal (fun o => match o with error.Return x => x | _ => b end)) in H.
+      subst b.
+      apply andb_prop in Hcond.
+      destruct Hcond as (H1, H2).
+      apply Z_to_two_compl_to_Z.
+      * apply Z.le_ge.
+        apply Z.geb_le.
+        assumption.
+      * apply Z.ltb_lt.
+        assumption.
+    + intro Hcond.
+      rewrite Hcond in H.
+      discriminate.
+Qed.
+
+Lemma of_Z_to_Z b : of_Z (to_Z b) = error.Return b.
+Proof.
+  rewrite <- of_Z_to_Z_eqv.
+  reflexivity.
 Qed.
 
 Definition compare (a b : int64) : comparison :=
@@ -61,6 +187,7 @@ Proof.
     apply (f_equal of_Z) in H.
     rewrite of_Z_to_Z in H.
     rewrite of_Z_to_Z in H.
-    assumption.
+    injection H.
+    auto.
   - apply f_equal.
 Qed.
